可以用的公式

位置表示法：  

$$d = \sum_{i=1}^{n}d_{i}r^{i-1}$$

分解因式：

$$b^{n}-1 = (b-1)(b^{n-1}+b^{n-2}+……+1)$$

负数表示(二进制)：
where $k$ is the number of bits for an integer:

$$Negative(x) = 2^{k} - x$$

证明二进制的负数（two‘s complement of X）等于 X 的 ones’complement ＋ 1（即，X每位求反加1）

$$x = \sum_{i=1}^{k}d_{i}2^{i-1}$$

$\because$ 
$$Negative(x) = 2^{k} - x$$,where $k$ is the number of bits for an integer.

$\therefore$ 
$$Negative(x) = 2^{k} - 1 - x + 1$$

$\because$ 
$$b^{n}-1 = (b-1)(b^{n-1}+b^{n-2}+……+1)$$

$\therefore$ 
$$2^{k} - 1 = (2 - 1)\sum_{i=1}^{k}2^{i-1}$$,that is $k$ bits 1.

$\because$ 
$$x + \overline{x} = 1$$,when $x$ is a binary number $0$ or $1$.

$\therefore$ 
$$Negative(x) = 2^{k} - x = \sum_{i=1}^{k}2^{i-1} - x + 1 = \sum_{i=1}^{k}\overline{x_{i}} + 1$$

$\blacksquare$


关于位拓展的证明，正数显然，以下证明负数：

$\because$ Positional Notation 

$${(x)}_{2} = \sum_{i=1}^{k}d_{i}2^{i-1}$$

$\because$ Two's complement 

$$N(x) = 2^{k} - x$$, where $k$ is the number of bits for an integer and,
$$N'(x) = 2^{m} - x$$,where $$m > k$$

$\therefore$ 
$$N'(x) = 2^{m} - x = (2^{m} - 2^{k}) + 2^{k} - x = (2^{m}-1) - (2^{k}-1) + N(x)$$

$\because$ 
$$b^{n}-1 = (b-1)(b^{n-1}+b^{n-2}+……+1)$$

$\therefore$ 
$$2^{m}-1 = (2-1)\sum_{i=1}^{m}2^{i-1}$$, that is $m$ bits $1$.

So the same, 
$$(2^{k}-1)$$ is $k$ bits $1$.

$\therefore$ 
$$N'(x) = (2^{m}-1) - (2^{k}-1) + N(x) = \sum_{i=k+1}^{m}2^i + N(x) = \sum_{i=k+1}^{m}2^i + \sum_{i=1}^{k}d_{i}2^{i-1}$$

$\therefore$ If N(x) is a negative binary integer, the most-significant bit can be repeated in all the extra bits.

$\blacksquare$

证明进制转换：$r_{0}$进制转化成$r$进制

$\because$ Positional Notation 

$$(d)_{r0} = \sum_{i=1}^{n}d_{i}r^{i-1}$$

$\therefore$ 
$$(d)_{r0} = \sum_{i=1}^{n}d_{i}r^{i-1}$$ 

= $$d_{n}r^{n-1} + d_{n-1}r^{n-2} + ··· + d_{3}r^{2} + d_{2}r + d_{1}$$ 

= $$r(d_{n}r^{n-2} +d_{n-1}r^{n-3} + ··· + d_{3}r + d_{2}) + d_{1}$$ 

= $$r(r(d_{n}r^{n-3} +d_{n-1}r^{n-4} + ··· + d_{4}r + d_{3}) + d_{2}) + d_{1}$$

In order to get every digit , we can use Modulo operation:

$\therefore$ 
$$(d)_{r0} (mod r) = d_{1}$$ 

$\because$ 
$$\frac{(d)_{r0}}{r} 
= (d_{n}r^{n-2} +d_{n-1}r^{n-3} + ··· + d_{3}r + d_{2}) + \frac{d_{1}}{r}$$

$\therefore$ 
$$[\frac{(d)_{r0}}{r}] (mod r) = d_{2}$$
